Comments!

theories/OGS/Strategy.v
@@ -1,3 +1,12 @@
+(*|
+The Machine Strategy (§ 5.3)
+============================
+
+Having defined the `OGS game <Game.html>`_ and axiomatized the
+`language machine <Machine.v>`_, we are now ready to construct the *machine strategy*.
+
+.. coq:: none
+|*)
 From OGS Require Import Prelude.
 From OGS.Utils Require Import Psh Rel.
 From OGS.Ctx Require Import All Ctx.
@@ -16,18 +25,19 @@ Reserved Notation "x ≈⟦ogs Δ ⟧≈ y" (at level 50).
 
 Section with_param.
 (*|
-We consider a language abstractly captured as a machine
+We consider a language abstractly captured as a machine.
 |*)
   Context `{CC : context T C} {CL : context_laws T C}.
   Context {val} {VM : subst_monoid val} {VML : subst_monoid_laws val}.
   Context {conf} {CM : subst_module val conf} {CML : subst_module_laws val conf}.
   Context {obs : obs_struct T C} {M : machine val conf obs}.
-
 (*|
-Active and passive OGS environments (Def 5.16)
-TODO comment
-Env M Δ Act Φ : environment part of the player (aka active at es) configuration at (Δ + es)
-Env M Δ Pas Φ : environment part of the opponent (aka passive at es) configuration at (Δ + es)
+We start off by defining active and passive OGS assignments (Def 5.16). This datastructure
+will hold the memory part of a strategy state, remembering the values which we have
+hidden from Opponent and given as fresh variables.
+
+.. coq::
+   :name: ogsenv
 |*)
   Inductive ogs_env (Δ : C) : polarity -> ogs_ctx -> Type :=
   | ENilA : ogs_env Δ Act ∅ₓ
@@ -35,19 +45,25 @@ Env M Δ Pas Φ : environment part of the opponent (aka passive at es) configura
   | EConA {Φ Γ} : ogs_env Δ Pas Φ -> ogs_env Δ Act (Φ ▶ₓ Γ)
   | EConP {Φ Γ} : ogs_env Δ Act Φ -> Γ =[val]> (Δ +▶ ↓⁺Φ) -> ogs_env Δ Pas (Φ ▶ₓ Γ)
   .
+(*|
+.. coq:: none
+|*)
   #[global] Arguments ENilA {Δ}.
   #[global] Arguments ENilP {Δ}.
   #[global] Arguments EConA {Δ Φ Γ} u.
   #[global] Arguments EConP {Δ Φ Γ} u γ.
   Derive Signature NoConfusion NoConfusionHom for ogs_env.
-
+(*|
+|*)
   Notation "'ε⁺'" := (ENilA).
   Notation "'ε⁻'" := (ENilP).
   Notation "u ;⁺" := (EConA u).
   Notation "u ;⁻ e" := (EConP u e).
-
 (*|
-Collapsing functions (Def 5.18)
+Next we define the collapsing function on OGS assignments (Def 5.18).
+
+.. coq::
+   :name: envcollapse
 |*)
   Equations collapse {Δ p Φ} : ogs_env Δ p Φ -> ↓[p^]Φ =[val]> (Δ +▶ ↓[p]Φ) :=
     collapse ε⁺       := ! ;
@@ -55,8 +71,13 @@ Collapsing functions (Def 5.18)
     collapse (u ;⁺)   := collapse u ⊛ᵣ r_cat3_1 ;
     collapse (u ;⁻ e) := [ collapse u , e ] .
   Notation "ₐ↓ γ" := (collapse γ).
-  #[derive(eliminator=no)]
+(*|
+We readily define the zipping function (Def 6.10).
 
+.. coq::
+   :name: zip
+|*)
+  #[derive(eliminator=no)]
   Equations bicollapse {Δ} Φ : ogs_env Δ Act Φ -> ogs_env Δ Pas Φ -> forall p, ↓[p]Φ =[val]> Δ :=
     bicollapse ∅ₓ       (ε⁺)     (ε⁻)     Act   := ! ;
     bicollapse ∅ₓ       (ε⁺)     (ε⁻)     Pas   := ! ;
@@ -64,7 +85,12 @@ Collapsing functions (Def 5.18)
           [ bicollapse Φ v u Pas , γ ⊛ [ a_id , bicollapse Φ v u Act ] ] ;
     bicollapse (Φ ▶ₓ _) (v ;⁺)   (u ;⁻ e) Pas := bicollapse Φ u v Act .
   #[global] Arguments bicollapse {Δ Φ} u v {p}.
+(*|
+And the fixpoint property linking collapsing and zipping (Prop 6.13).
 
+.. coq::
+   :name: collapsezip
+|*)
   Lemma collapse_fix_aux {Δ Φ} (u : ogs_env Δ Act Φ) (v : ogs_env Δ Pas Φ)
     :  ₐ↓u ⊛ [ a_id , bicollapse u v ] ≡ₐ bicollapse u v
      /\ ₐ↓v ⊛ [ a_id , bicollapse u v ] ≡ₐ bicollapse u v .
@@ -86,9 +112,12 @@ Collapsing functions (Def 5.18)
   Lemma collapse_fix_pas {Δ Φ} (u : ogs_env Δ Act Φ) (v : ogs_env Δ Pas Φ)
     : ₐ↓v ⊛ [ a_id , bicollapse u v ] ≡ₐ bicollapse u v .
   Proof. now apply collapse_fix_aux. Qed.
-
 (*|
-Alternative definition using precise lookup.
+Here we provide an alternative definition to the collapsing functions, using a more
+precisely typed lookup function. This is more practical to use when reasoning about
+the height of a variable, in the `eventual guardedness proof <CompGuarded.html>`_.
+
+First we compute actual useful subset of the context used by a particular variable.
 |*)
   Equations ctx_dom Φ p {x} : ↓[p^]Φ ∋ x -> C :=
     ctx_dom ∅ₓ       Act i with c_view_emp i := { | ! } ;
@@ -98,7 +127,9 @@ Alternative definition using precise lookup.
       | Vcat_l j := ctx_dom Φ Act j ;
       | Vcat_r j := ↓[Act]Φ } .
   #[global] Arguments ctx_dom {Φ p x} i.
-
+(*|
+Next we provide a renaming from this precise domain to the actual current allowed context.
+|*)
   Equations r_ctx_dom Φ p {x} (i : ↓[p^]Φ ∋ x) : ctx_dom i ⊆ ↓[p]Φ :=
     r_ctx_dom ∅ₓ       Act i with c_view_emp i := { | ! } ;
     r_ctx_dom ∅ₓ       Pas i with c_view_emp i := { | ! } ;
@@ -107,7 +138,10 @@ Alternative definition using precise lookup.
       | Vcat_l j := r_ctx_dom Φ Act j ;
       | Vcat_r j := r_id } .
   #[global] Arguments r_ctx_dom {Φ p x} i.
-
+(*|
+We can write this more precise lookup function, returning a value in just the necessary
+context.
+|*)
   Equations lookup {Δ p Φ} (γ : ogs_env Δ p Φ) [x] (i : ↓[p^]Φ ∋ x)
             : val (Δ +▶ ctx_dom i) x :=
     lookup ε⁺       i with c_view_emp i := { | ! } ;
@@ -116,7 +150,9 @@ Alternative definition using precise lookup.
     lookup (γ ;⁻ e) i with c_view_cat i := {
       | Vcat_l j := lookup γ j ;
       | Vcat_r j := e _ j } .
-
+(*|
+We relate the precise lookup with the previously defined collapse.
+|*)
   Lemma lookup_collapse {Δ p Φ} (γ : ogs_env Δ p Φ) :
     collapse γ ≡ₐ (fun x i => lookup γ i ᵥ⊛ᵣ [ r_cat_l , r_ctx_dom i ᵣ⊛ r_cat_r ]).
   Proof.
@@ -133,12 +169,16 @@ Alternative definition using precise lookup.
       cbn; rewrite a_ren_l_id, a_cat_id.
       symmetry; apply v_var_sub.
   Qed.
-
 (*|
-OGS strategies (Def 5.19)
+Machine Strategy (Def 5.19)
 ===========================
 
-Active and passive states
+We define active and passive states of the machine strategy. Active states consist of
+the pair of a language configuration and an active OGS assignement. Passive states consist
+solely of a passive OGS assignement.
+
+.. coq::
+   :name: machinestate
 |*)
   Record m_strat_act Δ (Φ : ogs_ctx) : Type := MS {
     ms_conf : conf (Δ +▶ ↓⁺Φ) ;
@@ -149,9 +189,15 @@ Active and passive states
   #[global] Arguments ms_env {Δ Φ}.
 
   Definition m_strat_pas Δ : psh ogs_ctx := ogs_env Δ Pas.
-
 (*|
-Action and reaction morphisms
+Next we define the action and reaction morphisms of the machine strategy. First
+``m_strat_wrap`` provides the active transition given an already evaluated normal form,
+such that the action morphism ``m_strat_play`` only has to evaluate the active part
+of the state. ``m_strat_resp`` mostly is a wrapper around ``oapp``, our analogue to
+the embedding from normal forms to language configurations present in the paper.
+
+.. coq::
+   :name: machineplay
 |*)
   Definition m_strat_wrap {Δ Φ} (γ : ogs_env Δ Act Φ)
      : nf _ _ (Δ +▶ ↓⁺ Φ) -> (obs∙ Δ + h_actv ogs_hg (m_strat_pas Δ) Φ) :=
@@ -170,9 +216,10 @@ Action and reaction morphisms
     := fun m =>
          {| ms_conf := (ₐ↓γ _ (m_var m) ᵥ⊛ᵣ r_cat3_1) ⊙ (m_obs m)⦗r_cat_rr ᵣ⊛ a_id⦘ ;
             ms_env := γ ;⁺ |} .
-
 (*|
-Strategies (unfolded)
+These action and reaction morphisms define a coalgebra, which we now embed into the
+final coalgebra by looping them coinductively. This constructs the indexed interaction
+tree arising from starting the machine strategy at a given state.
 |*)
    Definition m_strat {Δ} : m_strat_act Δ ⇒ᵢ ogs_act Δ :=
     cofix _m_strat Φ e :=
@@ -182,12 +229,15 @@ Strategies (unfolded)
           | inr (x ,' p) => VisF x (fun r : ogs_e.(e_rsp) _ => _m_strat _ (m_strat_resp p r))
           end)
          (m_strat_play e).
-
+(*|
+We also provide a wrapper for the passive version of the above map.
+|*)
   Definition m_stratp {Δ} : m_strat_pas Δ ⇒ᵢ ogs_pas Δ :=
     fun _ x m => m_strat _ (m_strat_resp x m).
-
 (*|
-Notions of equivalence.
+We define the notion of equivalence on machine-strategy states given by the weak
+bisimilarity of the induced infinite trees. There is an active version, and a passive
+version, working pointwise.
 |*)
   Definition m_strat_act_eqv {Δ} : relᵢ (m_strat_act Δ) (m_strat_act Δ) :=
     fun i x y => m_strat i x ≈ m_strat i y.
@@ -196,7 +246,9 @@ Notions of equivalence.
   Definition m_strat_pas_eqv {Δ} : relᵢ (m_strat_pas Δ) (m_strat_pas Δ) :=
     fun i x y => forall m, m_strat_resp x m ≈ₐ m_strat_resp y m .
   Notation "x ≈ₚ y" := (m_strat_pas_eqv _ x y).
-
+(*|
+A technical lemma explaining how the infinite strategy unfolds.
+|*)
   Lemma unfold_mstrat {Δ a} (x : m_strat_act Δ a) :
     m_strat a x
     ≊ subst_delay
@@ -220,22 +272,24 @@ Notions of equivalence.
       + now apply it_eq_t_equiv.
     - destruct q.
   Qed.
-
 (*|
-Injection of configurations into strategies
+Next we construct the initial states. The active initial state is given by simply a
+configuration from the language machine while a passive initial state is given by
+an assignment into the final context Δ.
 |*)
    Definition inj_init_act Δ {Γ} (c : conf Γ) : m_strat_act Δ (∅ₓ ▶ₓ Γ) :=
     {| ms_conf := c ₜ⊛ᵣ (r_cat_r ᵣ⊛ r_cat_r) ; ms_env := ε⁻ ;⁺ |}.
 
   Definition inj_init_pas {Δ Γ} (γ : Γ =[val]> Δ) : m_strat_pas Δ (∅ₓ ▶ₓ Γ) :=
     ε⁺ ;⁻ (γ ⊛ᵣ r_cat_l).
-
+(*|
+This defines a notion of equivalence on the configurations of the language: bisimilarity
+of the induced strategies.
+|*)
   Definition m_conf_eqv Δ : relᵢ conf conf :=
     fun Γ u v => inj_init_act Δ u ≈ₐ inj_init_act Δ v .
-
 (*|
-Definition of composition (not for general OGS (counter-)strategies, but a more
-precise version only for machine (counter-)strategies).
+Finally we define composition of two matching machine-strategy states.
 |*)
   Record reduce_t (Δ : C) : Type := RedT {
     red_ctx : ogs_ctx ;
@@ -246,7 +300,12 @@ precise version only for machine (counter-)strategies).
   #[global] Arguments red_ctx {Δ}.
   #[global] Arguments red_act {Δ}.
   #[global] Arguments red_pas {Δ}.
+(*|
+First the composition equation.
 
+.. coq::
+   :name: compeqn
+|*)
   Definition compo_body {Δ} (x : reduce_t Δ)
     : delay (reduce_t Δ + obs∙ Δ)
     := fmap_delay (fun r => match r with
@@ -255,12 +314,19 @@ precise version only for machine (counter-)strategies).
                   end)
                   (m_strat_play x.(red_act)).
   
+(*|
+Then its naive fixpoint.
+
+.. coq::
+   :name: componaive
+|*)
   Definition compo {Δ a} (u : m_strat_act Δ a) (v : m_strat_pas Δ a)
     : delay (obs∙ Δ)
     := iter_delay compo_body (RedT u v).
-
 End with_param.
-
+(*|
+Finally we expose a bunch of notations to make everything more readable.
+|*)
 #[global] Notation "'ε⁺'" := (ENilA).
 #[global] Notation "'ε⁻'" := (ENilP).
 #[global] Notation "u ;⁺" := (EConA u).
