theories/OGS/CompGuarded.v
@@ -1,15 +1,15 @@
 (*|
 Eventual guardedness of the composition
-==========================================
+=======================================
 
-We want to prove adequacy by unicity of solutions to the set of
-equations defining the composition. To do so, we rely on the
-notion of guarded iteration introduced in [ITree/Guarded].
-Through this file, we prove that the composition is indeed
-eventually guarded.
-As described in §6.2, the proof relies crucially on the [eval_app_not_var] assumption (Def 6.6).
+We want to prove adequacy by unicity of solutions to the set of equations defining the
+composition. To do so, we rely on the notion of guarded iteration introduced in
+`ITree/Guarded.v <Guarded.html>`_. Through this file, we prove that the composition is
+indeed eventually guarded. As described in §6.3, the proof relies crucially on the
+``eval_app_not_var`` assumption (Def 6.21).
+
+.. coq:: none
 |*)
-
 From OGS Require Import Prelude.
 From OGS.Utils Require Import Psh Rel.
 From OGS.Ctx Require Import All Ctx.
@@ -26,21 +26,23 @@ appropriate axiomatization.
   Context `{CC : context T C} {CL : context_laws T C}.
   Context {val} {VM : subst_monoid val} {VML : subst_monoid_laws val}.
   Context {conf} {CM : subst_module val conf} {CML : subst_module_laws val conf}.
-  Context {obs : obs_struct T C} {M : machine val conf obs} {ML : machine_laws val conf obs}.
-  Context {VV : var_assumptions val}.
+  Context {obs : obs_struct T C} {M : machine val conf obs}.
+  Context {ML : machine_laws val conf obs} {VV : var_assumptions val}.
 
   Notation ogs_ctx := (ogs_ctx (C:=C)).
-
 (*|
 A central elements in the proof lies in ensuring that there exists a unique solution
-to [compo_body]. Since the composition of strategies is defined as such a solution,
+to ``compo_body``. Since the composition of strategies is defined as such a solution,
 adequacy can be established by proving that evaluating and observing the substituted
-term is also a solution of [compo_body].
+term is also a solution of ``compo_body``.
 
-By [iter_evg_uniq], we know that eventually guarded equations admit a unique fixed point:
-we hence start by proving this eventual guardedness, captured in lemma [compo_body_guarded].
+By ``iter_evg_uniq``, we know that eventually guarded equations admit a unique fixed point:
+we hence start by proving this eventual guardedness, captured in lemma
+``compo_body_guarded``.
+
+This proof will among other be using an induction on the *age* of a variable, ie it's
+height in the OGS position Φ. We provide this definition and utilities.
 |*)
-
   Equations var_height Φ p {x} : ↓[p]Φ ∋ x -> nat :=
     var_height ∅ₓ       Pas i with c_view_emp i := { | ! } ;
     var_height ∅ₓ       Act i with c_view_emp i := { | ! } ;
@@ -75,7 +77,10 @@ we hence start by proving this eventual guardedness, captured in lemma [compo_bo
     var_height' i with c_view_cat i := {
       | Vcat_l j := O ;
       | Vcat_r j := var_height j } .
-
+(*|
+This is the main theorem about height: if we lookup a variable in an OGS environment and
+obtain another variable, then this new variable is strictly lower than the first one.
+|*)
   Lemma height_decrease {Δ Φ p} (v : ogs_env Δ p Φ) {x}
         (j : ↓[p^] Φ ∋ x)
         (H :  is_var (ₐ↓v _ j))
@@ -98,7 +103,12 @@ we hence start by proving this eventual guardedness, captured in lemma [compo_bo
       + dependent destruction v; clear Heqv0.
         revert j1; cbn; rewrite Heq; exact var_height_bound.
   Qed.
-
+(*|
+We are now ready to prove eventual guardedness. In fact the main lemma will have a slightly
+different statement, considering a particular kind of pair of OGS states: the ones we
+obtain when restarting after an interaction. As the statement is quite long we factor
+it in a definition first.
+|*)
   Definition compo_body_guarded_aux_stmt {Δ Φ} (u : ogs_env Δ Act Φ) (v : ogs_env Δ Pas Φ)
     {x} (o : obs x) (γ : dom o =[val]> (Δ +▶ ↓⁺ Φ)) (j : ↓⁺ Φ ∋ x) : Prop
     := ev_guarded
@@ -106,35 +116,47 @@ we hence start by proving this eventual guardedness, captured in lemma [compo_bo
          (compo_body (RedT (MS ((ₐ↓v _ j ᵥ⊛ᵣ r_cat3_1) ⊙ o⦗r_cat_rr ᵣ⊛ a_id⦘)
                                (v ;⁺))
                            (u ;⁻ γ))) .
-
+(*|
+Now the main proof.
+|*)
   Lemma compo_body_guarded_aux
     {Δ Φ} (u : ogs_env Δ Act Φ) (v : ogs_env Δ Pas Φ)
     {x} (o : obs x) γ j : compo_body_guarded_aux_stmt u v o γ j .
   Proof.
-    (* setup wf induction on no-infinite-redex *)
+(*|
+First we setup an induction on the accessibility of the current observation in the relation
+given by the "no-infinite redex" property.
+|*)
     revert Φ u v γ j.
     pose (o' := (x ,' o)); change x with (projT1 o'); change o with (projT2 o').
     generalize o'; clear x o o'; intro o.
     pose (wf := eval_app_not_var o); induction wf.
     destruct x as [ x o ]; cbn [ projT1 projT2 ] in *.
     clear H; rename H0 into IHred; intros Φ u v γ j.
-
-    (* setup wf induction on no-infinite var lookup *)
+(*|
+Next we setup an induction on the height of the current variable we have restarted on.
+|*)
     pose (h := lt_wf (var_height j)); remember (var_height j) as n.
     revert Φ u v γ j Heqn; induction h.
     clear H; rename x0 into n, H0 into IHvar; intros Φ u v γ j Heqn.
-
-    (* case: is lookup a variable? *)
+(*|
+Then we case split on whether ``ₐ↓ v x j`` is a variable or not.
+|*)
     unfold compo_body_guarded_aux_stmt.
     pose (vv := ₐ↓ v x j); fold vv.
     destruct (is_var_dec vv).
+(*|
+Case 1: it is a variable.
 
-    (* lookup is a var: either final or step on no-infinite var lookup *)
+First, some shenenigans to extract the variable.
+|*)
     - rewrite (is_var_get_eq i); unfold vv in *; clear vv.
       unfold v_ren; rewrite v_sub_var; unfold r_emb.
       unfold ev_guarded; cbn.
-
-      (* trickery to apply eval_nf_ret *)
+(*|
+Next, we are evaluating a normal form, so we know by hypothesis ``eval_nf_ret`` that it
+will reduce to the same normal form. We need some trickery to rewrite by this bisimilarity.
+|*)
       pose proof (Heval :=
                     eval_nf_ret ((r_cat3_1 x (is_var_get i)) ⋅ o ⦇ r_cat_rr ᵣ⊛ a_id  ⦈)).
       unfold comp_eq in Heval; apply it_eq_step in Heval.
@@ -150,18 +172,28 @@ we hence start by proving this eventual guardedness, captured in lemma [compo_bo
       unfold observe in x; rewrite <- x; clear x; cbn.
       unfold m_strat_wrap, r_cat3_1; cbn.
       remember (ₐ↓v _ j) as vv.
+(*|
+Now, we case split to see whether this variable was a final variable or one given by
+the opponent.
+|*)
       destruct i; cbn; destruct (c_view_cat i).
-
-      (* final channel, trivially guarded *)
+(*|
+In case of a final variable the composition is ended, hence guarded, hence eventually
+guarded.
+|*)
       + rewrite c_view_cat_simpl_l; now do 2 econstructor.
-
-      (* interaction, step on no-infinite var lookup *)
+(*|
+In the other case, there is an interaction. Since we have looked-up a variable and
+obtained another variable, we know it is strictly older and use our induction hypothesis
+on the height of the current variable.
+|*)
       + rewrite c_view_cat_simpl_r; cbn.
         refine (GNext _).
         unshelve refine (IHvar _ _ _ _ _ _ _ eq_refl).
         rewrite Heqn; clear Heqn; unfold cut_l.
-
-        (* trickery to apply height_decrease *)
+(*|
+There is some trickery to apply ``height_decrease``.
+|*)
         clear tt ttn a1 a.
         assert (i : is_var (ₐ↓v _ j)).
           rewrite <- Heqvv.
@@ -172,8 +204,12 @@ we hence start by proving this eventual guardedness, captured in lemma [compo_bo
         rewrite <- Heqvv; unfold var_height'.
         rewrite c_view_cat_simpl_l, c_view_cat_simpl_r; cbn.
         now apply Nat.lt_succ_diag_r.
-
-    (* lookup is not a var: step on no-infinite-redex *)
+(*|
+Case 2: the looked-up value is not a variable. In this case we look at one step of the
+evaluation. If there is a redex we are happy. Else, our resumed configuration was
+still a normal form and we can exhibit a proof of the bad instanciation relation, which
+enables us to call our other induction hypothesis.
+|*)
     - unfold ev_guarded; cbn.
       remember (eval ((vv ᵥ⊛ r_emb r_cat3_1) ⊙ o ⦗ r_cat_rr ᵣ⊛ a_id ⦘)) as tt.
       remember (_observe tt) as ot.
@@ -188,7 +224,10 @@ we hence start by proving this eventual guardedness, captured in lemma [compo_bo
       rewrite Heqtt in Heqot; rewrite <- Heqot.
       now econstructor.
   Qed.
-
+(*|
+Now the actual proof of eventual guardedness is just about unfolding a bit of the beginning
+of the interactions until we attain a resume and can apply our main lemma.
+|*)
   Lemma compo_body_guarded {Δ} : eqn_ev_guarded (fun 'T1_0 => compo_body (Δ := Δ)).
   Proof.
     intros [] [ Γ [ c u ] v ]; unfold m_strat_pas in v.
@@ -199,7 +238,11 @@ we hence start by proving this eventual guardedness, captured in lemma [compo_bo
     destruct (c_view_cat i); try now do 2 econstructor.
     refine (GNext _); apply compo_body_guarded_aux.
   Qed.
-
+(*|
+From the previous proof we can directly apply the strong fixed point construction on
+eventually guarded equations and obtain a composition operator without any ``Tau`` node
+at interaction points.
+|*)
   Definition compo_ev_guarded {Δ a} (u : m_strat_act Δ a) (v : m_strat_pas Δ a)
     : delay (obs∙ Δ)
     := iter_ev_guarded _ compo_body_guarded T1_0 (RedT u v).
