theories/OGS/Game.v
@@ -2,7 +2,6 @@
 The OGS Game (§ 5.1 and 5.2)
 ==============================
 |*)
-
 From OGS Require Import Prelude.
 From OGS.Utils Require Import Rel.
 From OGS.Ctx Require Import All Ctx.
@@ -12,26 +11,32 @@ From OGS.ITree Require Import Event ITree.
 Reserved Notation "↓⁺ Ψ" (at level 9).
 Reserved Notation "↓⁻ Ψ" (at level 9).
 Reserved Notation "↓[ p ] Ψ" (at level 9).
-
 (*|
 Games (§ 5.1)
 ===============
-Levy and Staton's general notion of game.
-|*)
 
-(*|
+Levy and Staton's general notion of game.
+
 An half games (Def 5.1) is composed of "moves" as an indexed family of types,
-and a [next] map computing the next index following a move.
+and a "next" map computing the next index following a move.
+
+.. coq::
+   :name: halfgame
 |*)
 Record half_game (I J : Type) := {
  g_move : I -> Type ;
  g_next : forall i, g_move i -> J
 }.
+(*|
+.. coq:: none
+|*)
 Arguments g_move {I J h} i.
 Arguments g_next {I J h i} m.
-
 (*|
 Action (h_actv) and reaction (h_pasv) functors (Def 5.8)
+
+.. coq::
+   :name: actionreaction
 |*)
 Definition h_actv {I J} (H : half_game I J) (X : psh J) : psh I :=
   fun i => { m : H.(g_move) i & X (H.(g_next) m) } .
@@ -48,24 +53,33 @@ Definition h_pasvR {I J} (H : half_game I J) {X Y : psh J} (R : relᵢ X Y)
 
 (*|
 A game (Def 5.4) is composed of two compatible half games.
+
+.. coq::
+   :name: game
 |*)
 Record game (I J : Type) : Type := {
   g_client : half_game I J ;
   g_server : half_game J I
 }.
+(*|
+.. coq:: none
+|*)
 Arguments g_client {I J}.
 Arguments g_server {I J}.
-
+(*|
+Given a game, we can construct an ``event``. See `ITree/Event.v <Event.html>`_
+|*)
 Definition e_of_g {I J} (G : game I J) : event I I :=
   {| e_qry := fun i => G.(g_client).(g_move) i ;
      e_rsp := fun i q => G.(g_server).(g_move) (G.(g_client).(g_next) q) ;
      e_nxt := fun i q r => G.(g_server).(g_next) r |} .
-
 (*|
-OGS Games (§ 5.2)
-==================
-|*)
+The OGS Game (§ 5.2)
+====================
 
+First let us define a datatype for polarities, active and passive (called "waiting") in
+the paper.
+|*)
 Variant polarity : Type := Act | Pas .
 Derive NoConfusion for polarity.
 
@@ -76,15 +90,23 @@ Equations p_switch : polarity -> polarity :=
 
 Section with_param.
 (*|
-We consider an observation structure.
+We consider an observation structure, given by a set of types ``T``, a notion of contexts
+``C`` and a operator giving the observations and their domain. See
+`Ctx/Family.v <Family.html#oper>`_ and `OGS/Obs.v <Obs.html>`_.
 |*)
   Context `{CC : context T C} {obs : obs_struct T C}.
-
-  Definition ogs_ctx := ctx C.
-
 (*|
-Interleaved contexts (Def 5.12)
-Collapsing functions (Def 5.13)
+Interleaved contexts (Def 5.12) are given by the free context structure over ``C``.
+
+.. coq::
+   :name: ogsctx
+|*)
+  Definition ogs_ctx := ctx C.
+(*|
+We define the collapsing functions (Def 5.13).
+
+.. coq::
+   :name: ctxcollapse
 |*)
   Equations join_pol : polarity -> ogs_ctx -> C :=
     join_pol Act ∅ₓ       := ∅ ;
@@ -95,9 +117,11 @@ Collapsing functions (Def 5.13)
   Notation "↓⁺ Ψ" := (join_pol Act Ψ).
   Notation "↓⁻ Ψ" := (join_pol Pas Ψ).
   Notation "↓[ p ] Ψ" := (join_pol p Ψ).
-
 (*|
-Half games and games (Def 5.15)
+Finally we define the OGS half-game and game (Def 5.15).
+
+.. coq::
+   :name: ogsgame
 |*)
   Definition ogs_hg : half_game ogs_ctx ogs_ctx :=
     {| g_move Ψ := obs∙ ↓⁺Ψ ;
@@ -106,9 +130,16 @@ Half games and games (Def 5.15)
   Definition ogs_g : game ogs_ctx ogs_ctx :=
     {| g_client := ogs_hg ;
        g_server := ogs_hg  |} .
-
+(*|
+We define the event of OGS moves.
+|*)
   Definition ogs_e : event ogs_ctx ogs_ctx := e_of_g ogs_g.
+(*|
+And finally we define active OGS strategies and passive OGS strategies.
 
+.. coq::
+   :name: ogsstrat
+|*)
   Definition ogs_act (Δ : C) : psh ogs_ctx := itree ogs_e (fun _ => obs∙ Δ).
   Definition ogs_pas (Δ : C) : psh ogs_ctx := h_pasv ogs_hg (ogs_act Δ).
 
