theories/OGS/Machine.v
@@ -1,20 +1,25 @@
 (*|
-Evaluation Structure (Definition 4.7)
-=======================================
-Abstract characterization of the evaluation structure of a programming
-language.
-We have here a minor mismatch between the formalization and the paper:
+Evaluation structure and language machine
+=========================================
+
+In this file we pull everything together and define evaluation structures and
+the abstract characterization of a language machine, together with all the associated
+laws.
+
+Note that we have here a minor mismatch between the formalization and the paper:
 we have realized a posteriori a more elegant way to decompose the abstract
 machine as exposed in the paper.
-Here, instead of only requiring an embedding of normal forms into configurations,
-we require an application function describing how to rebuild a configuration
-from a value, an observation, and an assignment.
-This less minimalist axiomatization puts the dependencies of our modules slightly
-backwards compared to the paper's Section 4.
-Here, evaluation structures, dubbed [machine]s, are parameterized by a substitution
-monoid of values, a substitution module of configurations, and an observation structure, instead of coming first.
 
-Patching the development for following the paper's presentation would be slightly
+Here, instead of only requiring an embedding of normal forms into configurations,
+we require an application function ``oapp`` describing how to rebuild a configuration
+from a value, an observation, and an assignment. This less minimalist axiomatization puts
+the dependencies of our modules slightly backwards compared to the paper's Section 4.
+
+Here, evaluation structures, dubbed ``machines``, are parameterized by a substitution
+monoid of values, a substitution module of configurations, and an observation structure,
+instead of coming first.
+
+Patching the development to follow more closely the paper's presentation would be slightly
 technical due to the technicality of the mechanized proofs involved, but essentially
 straightforward.
 
@@ -28,32 +33,57 @@ From OGS.ITree Require Import Event Eq Delay.
 
 Section with_param.
   Context `{CC : context T C}.
-
 (*|
-Evaluation structures, telling us how to evaluate a configuration,
-and how to stitch one back together from the data sent by Opponent.
+We here define what is called an evaluation structure in the paper (Def 4.7). It tells
+us how to evaluate a configuration to a normal form and how to stitch one back together
+from the data sent by Opponent. 
+
+.. coq::
+   :name: machine
 |*)
 Class machine (val : Fam₁ T C) (conf : Fam₀ T C) (obs : obs_struct T C) := {
   eval : conf ⇒₀ (delay ∘ nf obs val) ;
   oapp [Γ x] (v : val Γ x) (o : obs x) : dom o =[val]> Γ -> conf Γ ;
 }.
+(*|
+.. coq:: none
+|*)
 #[global] Arguments eval {_ _ _ _} [_].
 #[global] Arguments oapp {_ _ _ _} [_ _].
+(*|
+Next we define "evaluating then observing".
 
+.. coq::
+   :name: evalobs
+|*)
 Definition evalₒ `{machine val conf obs}
   : conf ⇒₀ (delay ∘ obs∙) :=
   fun _ t => then_to_obs (eval t) .
+(*|
+.. coq:: none
+|*)
 #[global] Arguments evalₒ {_ _ _ _} [_].
-
+(*|
+|*)
 Notation "v ⊙ o ⦗ a ⦘" := (oapp v o a) (at level 20).
+(*|
+We can readily define the embedding from normal forms to configurations.
 
+.. coq::
+   :name: embed
+|*)
 Definition emb `{machine val conf obs} {_ : subst_monoid val}
   : nf obs val ⇒₀ conf
   := fun _ n => oapp (v_var (nf_var n)) (nf_obs n) (nf_args n) .
-#[global] Arguments emb {_ _ _ _ _} [_].
-
 (*|
-The ≺ relation (Def 6.7)
+.. coq:: none
+|*)
+#[global] Arguments emb {_ _ _ _ _} [_].
+(*|
+Next we define the "bad instanciation" relation (Def 6.21).
+
+.. coq::
+   :name: badinst
 |*)
 Variant head_inst_nostep `{machine val conf obs} {VM : subst_monoid val} 
         (u : sigT obs) : sigT obs -> Prop :=
@@ -61,50 +91,44 @@ Variant head_inst_nostep `{machine val conf obs} {VM : subst_monoid val}
     : ¬(is_var v)
     -> evalₒ (v ⊙ o⦗a⦘) ≊ ret_delay (i ⋅ projT2 u)
     -> head_inst_nostep u (y ,' o) .
-
 (*|
-Axiomatization of the machine
+Finally we define the structure containing all the remaining axioms of a language
+machine.
 |*)
 Class machine_laws val conf obs {M : machine val conf obs} {VM : subst_monoid val}
       {CM : subst_module val conf} := {
-
 (*|
-[app] respects [asgn_eq], to avoid relying on functional extensionality
+``oapp`` respects pointwise equality of assignments.
 |*)
    oapp_proper {Γ x} {v : val Γ x} {o} :: Proper (asgn_eq (dom o) Γ ==> eq) (oapp v o) ;
-
 (*|
-[app] commutes with substitution
+``oapp`` commutes with substitutions, presented as part of "evaluation respects
+substitution" (Def 4.26) in the paper.
 |*)
    app_sub {Γ1 Γ2 x} (v : val Γ1 x) (o : obs x) (a : dom o =[val]> Γ1) (b : Γ1 =[val]> Γ2)
    : (v ⊙ o⦗a⦘) ₜ⊛ b = (v ᵥ⊛ b) ⊙ o⦗a ⊛ b⦘ ;
-
 (*|
-Core hypothesis over the evaluator (Def 4.23): "Substituting, then evaluating"
-is equivalent to "Evaluating, then substituting, then evaluating once more"
+Second part of "evaluation respects substitution". This is the core hypothesis of the OGS
+soundness, stating essentially "substituting, then evaluating" is equivalent to
+"evaluating, then substituting, then evaluating once more".
 |*)
    eval_sub {Γ Δ} (c : conf Γ) (a : Γ =[val]> Δ)
    : eval (c ₜ⊛ a) ≋ bind_delay' (eval c) (fun n => eval (emb n ₜ⊛ a)) ;
-
 (*|
 Evaluating the embedding of a normal form is equivalent to returning the normal
-form (Def. 4.7)
+form. This is part of the evaluation structure (Def. 4.7) in the paper.
 |*)
    eval_nf_ret {Γ} (u : nf obs val Γ)
    : eval (emb u) ≋ ret_delay u ;
-
 (*|
-The machine has finite redexes (§ 6.2). Necessary for establishing that the composition
-can be defined by eventually guarded iteration.
+At last the mystery hypothesis, stating that the machine has finite redexes (Def. 6.21).
+It is necessary for establishing that the composition can be defined by eventually
+guarded iteration.
 |*)
     eval_app_not_var : well_founded head_inst_nostep ;
   } .
-
-(*
-  Definition app' {Γ Δ} (u : Γ ⇒ᵥ Δ) (v : nf∙ Γ) : conf Δ :=
-    app (u _ (nf'_var v)) (nf'_obs v) (u ⊛ nf'_val v) .
-*)
-
 End with_param.
-
+(*|
+Finally we define a cute notation for applying an observation to a value.
+|*)
 #[global] Notation "v ⊙ o ⦗ a ⦘" := (oapp v o a) (at level 20).
