theories/OGS/Obs.v
@@ -1,3 +1,24 @@
+(*|
+Observation Structure (§ 4.4)
+=============================
+
+The messages that player and opponent exchange in the OGS
+arise from splitting normal forms into the head variable
+on which it is stuck, an observation, and an assignment.
+An *observation structure* axiomatizes theses observations
+of the language. They consist of:
+
+- a family `o_obs` indexed by the types of the language and,
+- a projection from observations to contexts of the language.
+
+In fact as these make sense quite generally, we have already defined
+them along with generic combinators on sorted families in
+`Ctx/Family.v <Family.html>`_. Much of the content of this file will
+be to wrap these generic definitions with more suitable names and
+provide specific utilities on top.
+
+.. coq:: none
+|*)
 From OGS Require Import Prelude.
 From OGS.Utils Require Import Rel.
 From OGS.Ctx Require Import All.
@@ -8,34 +29,40 @@ Open Scope ctx_scope.
 Reserved Notation "O ∙" (at level 5).
 Reserved Notation "'dom∙' o" (at level 5).
 Reserved Notation "u ≋ v" (at level 40).
-
 (*|
-Observation Structure (§ 4.4)
-==============================
+As explained above, observation structures are just `operators <Family.html#oper>`_. We
+rename their domain ``o_dom`` to just ``dom``.
 
-The messages that player and opponent exchange in the OGS
-arise from splitting normal forms into the head variable
-on which it is stuck, an observation, and an assignment.
-
-An **observation structure** axiomatizes the observations
-of the language:
-- a Type [typ] of types (assumed globally in §4),
-- a type-indexed set [obs] of observations,
-- a map [dom] mapping observations to values filling their copattern
-
+.. coq::
+   :name: obsstruct
 |*)
 #[global] Notation obs_struct T C := (Oper T C).
 #[global] Notation dom := o_dom.
+(*|
+Pointed observations consist of a pair of a variable and a matching observation.
+We construct them using the generic formal cut combinator on families defined
+in `Ctx/Family.v <Family.html#formalcut>`_.
+|*)
 Definition pointed_obs `{CC : context T C} (O : Oper T C) : Fam₀ T C
   := c_var ∥ₛ ⦉O⦊.
 #[global] Notation "O ∙" := (pointed_obs O).
 #[global] Notation m_var o := (o.(cut_l)).
 #[global] Notation m_obs o := (o.(cut_r)).
 #[global] Notation m_dom o := (o_dom o.(cut_r)).
+(*|
+Next we define normal forms, as triplets of a variable, an observation
+and an assignment filling the domain of the observation. For this we again
+use the formal cut combinator and the "observation filling" combinator,
+defined in `Ctx/Assignment.v <Assignment.html#filledop>`_.  
 
+.. coq::
+   :name: nf
+|*)
 Definition nf `{CC : context T C} (O : obs_struct T C) (X : Fam₁ T C) : Fam₀ T C
   := c_var ∥ₛ (O # X).
-
+(*|
+We now define two utilities for projecting normal forms to pointed observations.
+|*)
 Definition nf_to_obs `{CC : context T C} {O} {X : Fam₁ T C} : forall Γ, nf O X Γ -> O∙ Γ
   := f_cut_map f_id₁ forget_args.
 #[global] Coercion nf_to_obs : nf >-> pointed_obs.
@@ -43,7 +70,9 @@ Definition nf_to_obs `{CC : context T C} {O} {X : Fam₁ T C} : forall Γ, nf O 
 Definition then_to_obs `{CC : context T C} {O} {X : Fam₁ T C} {Γ}
   : delay (nf O X Γ) -> delay (O∙ Γ)
   := fmap_delay (nf_to_obs Γ).
-
+(*|
+Next, we define shortcuts for projecting normal forms into their various components.
+|*)
 Section with_param.
   Context `{CC : context T C} {O : obs_struct T C} {X : Fam₁ T C}.
 
@@ -57,7 +86,11 @@ Section with_param.
     := dom n.(cut_r).(fill_op).
   Definition nf_args {Γ} (n : nf O X Γ) : nf_dom n =[X]> Γ
     := n.(cut_r).(fill_args).
-
+(*|
+As normal forms contain an assignment, Coq's equality is not the right notion of
+equivalence: we wish to consider two normal forms as equivalent even if their assignment
+are merely *pointwise equal*.
+|*)
   Variant nf_eq {Γ} : nf O X Γ -> nf O X Γ -> Prop :=
   | NfEq {t} {i : Γ ∋ t} {o a1 a2} : a1 ≡ₐ a2 -> nf_eq (i⋅o⦇a1⦈) (i⋅o⦇a2⦈).
 
@@ -69,7 +102,9 @@ Section with_param.
     - intros ??? [] h2; dependent induction h2.
       econstructor; now transitivity a2.
   Qed.
-
+(*|
+We lift this notion of equivalence to computations returning normal forms.
+|*)
   Definition comp_eq {Γ} : relation (delay (nf O X Γ))
     := it_eq (fun _ : T1 => nf_eq) (i := T1_0).
 
