theories/OGS/Soundness.v
@@ -1,16 +1,14 @@
 (*|
 Soundness (Theorem 6.12)
 ========================
+
 Finally, all the pieces are in place to prove that bisimilarity of induced LTS is sound
-w.r.t. substitution equivalence.
-Having worked hard to establish adequacy and congruence of weak bisimilarity for composition,
-very little remains to do here.
+w.r.t. substitution equivalence. Having worked hard to establish
+`adequacy <Adequacy.html>`_ and `congruence <Congruence.html>`_
+of weak bisimilarity for composition, very little remains to do here.
 
-At the end of the file, we run two commands:
-- [About ogs_correction.] explicit the assumptions of the theorem, that we show how to instantiate in the [Example] folder on several concrete examples of languages.
-- [Print Assumptions ogs_correction.] explicit if any axiom has been used to establish the result. As stated in the Readme, we exclusively use [Eqdep.Eq_rect_eq.eq_rect_eq] (i.e., axiom K).
+.. coq:: none
 |*)
-
 From Coinduction Require Import coinduction.
 
 From OGS Require Import Prelude.
@@ -28,33 +26,68 @@ appropriate axiomatization.
   Context {conf} {CM : subst_module val conf} {CML : subst_module_laws val conf}.
   Context {obs : obs_struct T C} {M : machine val conf obs} {ML : machine_laws val conf obs}.
   Context {VV : var_assumptions val}.
-
 (*|
-Substitution equivalence of two abstract machine configurations (Def 4.21)
-|*)
-  Definition ciu {Γ} Δ (a b : conf Γ) : Prop
-    := forall γ : Γ =[val]> Δ, evalₒ (a ₜ⊛ γ) ≈ evalₒ (b ₜ⊛ γ).
-  Notation "x ≈⟦ciu Δ ⟧≈ y" := (ciu Δ x y) (at level 50).
+We define substitution equivalence of two language machine configurations (Def 4.24).
 
+.. coq::
+   :name: substeq
+|*)
+  Definition substeq {Γ} Δ (a b : conf Γ) : Prop
+    := forall γ : Γ =[val]> Δ, evalₒ (a ₜ⊛ γ) ≈ evalₒ (b ₜ⊛ γ).
+  Notation "x ≈⟦sub Δ ⟧≈ y" := (substeq Δ x y) (at level 50).
+(*|
+We define an intermediate notion of equivalence, stating that for any assignment ``γ``,
+the induced LTS are bisimilar when composed with the passive interpretation of ``γ``.
+|*)
   Definition barb {Γ} Δ (x y : conf Γ) : Prop
     := forall γ : Γ =[val]> Δ,
          (inj_init_act Δ x ∥ inj_init_pas γ)
        ≈ (inj_init_act Δ y ∥ inj_init_pas γ).
   Notation "x ≈⟦barb Δ ⟧≈ y" := (barb Δ x y) (at level 50).
-
-  Theorem barb_correction {Γ} Δ (x y : conf Γ) : x ≈⟦barb Δ ⟧≈ y -> x ≈⟦ciu Δ ⟧≈ y.
+(*|
+Barbed equivalence is sound w.r.t. substitution equivalence, by swapping the naive
+composition with the guarded one and then applying adequacy.
+|*)
+  Theorem barb_correction {Γ} Δ (x y : conf Γ) : x ≈⟦barb Δ ⟧≈ y -> x ≈⟦sub Δ ⟧≈ y.
   Proof.
     intros H e.
     rewrite (it_eq_wbisim _ _ _ (adequacy x e)), (it_eq_wbisim _ _ _ (adequacy y e)).
     unfold compo_ev_guarded; rewrite 2 iter_evg_iter; apply H.
   Qed.
+(*|
+Our main theorem: bisimilarity of induced OGS machine strategies is sound w.r.t.
+substitution equivalence, by applying barbed equivalence soundness, swapping the naive
+composition with the `opaque one <Congruence.html>`_ and then applying congruence.
 
-  Theorem ogs_correction {Γ} Δ (x y : conf Γ) : x ≈⟦ogs Δ ⟧≈ y -> x ≈⟦ciu Δ ⟧≈ y.
+.. coq::
+   :name: soundness
+|*)
+  Theorem ogs_correction {Γ} Δ (x y : conf Γ) : x ≈⟦ogs Δ ⟧≈ y -> x ≈⟦sub Δ ⟧≈ y.
   Proof.
     intro H; apply barb_correction.
     intro e; unfold compo.
     rewrite <- 2 (compo_compo_alt (x := RedT _ _)).
     apply compo_alt_proper; [ exact H | intro; reflexivity ].
   Qed.
-
 End with_param.
+(*|
+If you wish to double check these results you can run the following commands at
+this point in the file:
+
+.. coq::
+
+   About ogs_correction.
+   Print Assumptions ogs_correction.
+
+The first command will explicit the assumptions of the theorem, which we show how
+to provide with several examples:
+
+- `simply-typed call-by-value λ-calculus <STLC_CBV.html>`_
+- `untyped pure call-by-value λ-calculus <ULC_CBV.html>`_
+- `call-by-value System L <SystemL_CBV.html>`_
+- `polarized System D <SystemD.html>`_
+
+The second command will explicit if any axiom has been used to establish the
+result. As stated in the `prelude <Prelude.html>`_, we exclusively use
+:coqid:`Coq.Eqdep.Eq_rect_eq.eq_rect_eq`, ie Streicher's axiom K.
+|*)
